
module test.test where

data ℕ : Set where
  zero : ℕ
  suc  : ℕ → ℕ

{-# BUILTIN NATURAL ℕ #-}

import Relation.Binary.PropositionalEquality as Eq
open Eq using (_≡_; refl)
open Eq.≡-Reasoning using (begin_; _≡⟨⟩_; _∎)

_+_ : ℕ → ℕ → ℕ
zero + n = n
suc m + n = suc (m + n)

_*_ : ℕ → ℕ → ℕ
zero * n = 0
suc m * n = n + (m * n)

data Bin : Set where
  ⟨⟩ : Bin
  _O : Bin → Bin
  _I : Bin → Bin

inc : Bin → Bin
inc ⟨⟩ = ⟨⟩ O
inc (n O) = n I
inc (n I) = (inc n) O

to : ℕ → Bin
to zero = ⟨⟩ O
to (suc n) = inc (to n)

from : Bin → ℕ
from ⟨⟩ = 0
from (b O) = 2 * from b
from (b I) = 2 * suc (from b)
